HOL/testItreeScript.sml
@@ -20,7 +20,7 @@
  *
  * One possible reasoning method:
  * 1. express a clear (tauless) decomposition of the spec w/ conditions on FFI
- * 3. prove equivalence to the actual program semantics via weak bisimulation
+ * 2. prove equivalence to the actual program semantics via weak bisimulation
  *
  * future work: ideally we want some way of automatically unfolding/executing a
  * program, to easily show facts about its interaction tree directly. This should
@@ -32,10 +32,7 @@
  *)
 
 open HolKernel boolLib bossLib BasicProvers;
-open arithmeticTheory;
 open itreeTauTheory;
-open panSemTheory; (* eval_def *)
-open panItreeSemTheory;
 
 (* open monadsyntax; *)
 (* val _ = *)
@@ -46,8 +43,15 @@ open panItreeSemTheory;
 (*     ) *)
 (* val _ = monadsyntax.temp_enable_monad "itree_monad"; *)
 
-val _ = temp_set_fixity "↻" (Infixl 500);
-Overload "↻" = “itree_iter”;
+Definition itree_trigger_def:
+  itree_trigger event = Vis event Ret
+End
+Overload emit[local] = “itree_trigger”;
+Overload bind[local] = “itree_bind”;
+Overload iter[local] = “itree_iter”;
+
+val _ = temp_set_fixity "≈" (Infixl 500);
+Overload "≈" = “itree_wbisim”;
 
 (* these are useful ONLY for bisimulation *)
 val or1_tac = disj1_tac
@@ -59,13 +63,6 @@ val or4_tac = disj2_tac >> disj2_tac >> disj2_tac;
    itree_unfold f is the final (coinductive) arrow to the capital algebra
    where f = structure map (into primed itree), seed = itree algebra instance
  *)
-
-Overload trigger[local] = “itree_trigger”;
-Theorem trigger:
-  trigger event = Vis event Ret
-Proof
-  rw[itree_trigger_def]
-QED
 
 Theorem spin_unfold:
   spin = Tau spin
@@ -98,21 +95,21 @@ QED
    just to have a richer equational theory for wbisim
  *)
 
-Theorem itree_bind_trigger:
-  ⋆ (trigger e) k = Vis e k
+Theorem itree_bind_emit:
+  bind (emit e) k = Vis e k
 Proof
   rw[itree_trigger_def, itree_bind_thm, FUN_EQ_THM]
 QED
 
 Theorem itree_wbisim_vis:
-  ∀e k1 k2. (∀r. ≈ (k1 r) (k2 r)) ⇒ ≈ (Vis e k1) (Vis e k2)
+  ∀e k1 k2. (∀r. k1 r ≈ k2 r) ⇒ Vis e k1 ≈ Vis e k2
 Proof
   metis_tac[strip_tau_cases, itree_wbisim_cases]
 QED
 
 (* TODO itree_wbisim_tau is overloaded! merged. change later *)
 Theorem itree_wbisim_tau_eq:
-  ∀ t. ≈ (Tau t) t
+  ∀ t. (Tau t) ≈ t
 Proof
   qspecl_then [‘λa b. a = Tau b’] strip_assume_tac itree_wbisim_strong_coind >>
   strip_tac >>
@@ -124,11 +121,11 @@ Proof
 QED
 
 Triviality itree_wbisim_coind_upto_equiv:
-  ∀R t t'. ≈ t t'
-           ⇒ (∃t2 t3. t = Tau t2 ∧ t' = Tau t3 ∧ (R t2 t3 ∨ ≈ t2 t3)) ∨
+  ∀R t t'. t ≈ t'
+           ⇒ (∃t2 t3. t = Tau t2 ∧ t' = Tau t3 ∧ (R t2 t3 ∨ t2 ≈ t3)) ∨
              (∃e k k'.
                strip_tau t (Vis e k) ∧ strip_tau t' (Vis e k') ∧
-               ∀r. R (k r) (k' r) ∨ ≈ (k r) (k' r)) ∨
+               ∀r. R (k r) (k' r) ∨ k r ≈ k' r) ∨
              (∃r. strip_tau t (Ret r) ∧ strip_tau t' (Ret r))
 Proof
   metis_tac[itree_wbisim_cases]
@@ -161,12 +158,12 @@ QED
 
 (* Q.AP_TERM or AP_THM to lift eq *)
 Theorem itree_bind_strip_tau_wbisim:
-  ∀u u' k. strip_tau u u' ⇒ ≈ (⋆ u k) (⋆ u' k)
+  ∀u u' k. strip_tau u u' ⇒ bind u k ≈ bind u' k
 Proof
   Induct_on ‘strip_tau’ >>
   rpt strip_tac >-
    (CONV_TAC $ RATOR_CONV $ ONCE_REWRITE_CONV[itree_bind_thm] >>
-    ‘≈ (⋆ u k) (⋆ u' k)’ suffices_by
+    ‘bind u k ≈ bind u' k’ suffices_by
       metis_tac[itree_wbisim_trans, itree_wbisim_sym, itree_wbisim_tau_eq] >>
     rw[]) >-
    rw[itree_wbisim_refl] >>
@@ -175,7 +172,8 @@ QED
 
 (* note a similar theorem does NOT hold for Ret because bind expands to (k x) *)
 Theorem itree_bind_vis_strip_tau:
-  ∀u k k' e. strip_tau u (Vis e k') ⇒ strip_tau (⋆ u k) (Vis e (λx. ⋆ (k' x) k))
+  ∀u k k' e. strip_tau u (Vis e k')
+           ⇒ strip_tau (bind u k) (Vis e (λx. bind (k' x) k))
 Proof
   strip_tac >> strip_tac >> strip_tac >> strip_tac >>
   Induct_on ‘strip_tau’ >>
@@ -184,27 +182,27 @@ Proof
 QED
 
 Triviality itree_bind_vis_tau_wbisim:
-  ≈ (Vis a g) (Tau u)
+  Vis a g ≈ Tau u
   ⇒ (∃e k' k''.
-      strip_tau (⋆ (Vis a g) k) (Vis e k') ∧
-      strip_tau (⋆ (Tau u) k) (Vis e k'') ∧
-      ∀r. (∃t1 t2. ≈ t1 t2 ∧ k' r = ⋆ t1 k ∧ k'' r = ⋆ t2 k) ∨
-          ≈ (k' r) (k'' r))
+      strip_tau (bind (Vis a g) k) (Vis e k') ∧
+      strip_tau (bind (Tau u) k) (Vis e k'') ∧
+      ∀r. (∃t1 t2. t1 ≈ t2 ∧ k' r = bind t1 k ∧ k'' r = bind t2 k) ∨
+          k' r ≈ k'' r)
 Proof
   rpt strip_tac >>
   rw[itree_bind_thm] >>
   fs[Once itree_wbisim_cases] >>
   fs[Once $ GSYM itree_wbisim_cases] >>
-  qexists_tac ‘(λx. ⋆ (k' x) k)’ >>
+  qexists_tac ‘(λx. bind (k' x) k)’ >>
   rw[itree_bind_vis_strip_tau] >>
   metis_tac[]
 QED
 
 Theorem itree_bind_resp_t_wbisim:
-  ∀a b k. (≈ a b) ⇒ (≈ (⋆ a k) (⋆ b k))
+  ∀a b k. a ≈ b ⇒ bind a k ≈ bind b k
 Proof
   rpt strip_tac >>
-  qspecl_then [‘λa b. ∃t1 t2. (≈ t1 t2) ∧ a = (⋆ t1 k) ∧ b = (⋆ t2 k)’]
+  qspecl_then [‘λa b. ∃t1 t2. t1 ≈ t2 ∧ a = (bind t1 k) ∧ b = (bind t2 k)’]
               strip_assume_tac itree_wbisim_coind_upto >>
   pop_assum irule >>
   rw[] >-
@@ -222,7 +220,7 @@ Proof
       irule itree_bind_strip_tau_wbisim >>
       fs[Once itree_wbisim_cases]) >-
      (rw[itree_bind_thm] >>
-      ‘≈ u u'’ by metis_tac[itree_wbisim_tau, itree_wbisim_sym] >>
+      ‘u ≈ u'’ by metis_tac[itree_wbisim_tau, itree_wbisim_sym] >>
       metis_tac[]) >-
      (metis_tac[itree_wbisim_sym, itree_bind_vis_tau_wbisim]) >-
      (fs[Once itree_wbisim_cases]) >-
@@ -232,10 +230,10 @@ Proof
 QED
 
 Theorem itree_bind_resp_k_wbisim:
-  ∀t k1 k2. (∀r. ≈ (k1 r) (k2 r)) ⇒ (≈ (⋆ t k1) (⋆ t k2))
+  ∀t k1 k2. (∀r. k1 r ≈ k2 r) ⇒ bind t k1 ≈ bind t k2
 Proof
   rpt strip_tac >>
-  qspecl_then [‘λa b. ∃t. a = (⋆ t k1) ∧ b = (⋆ t k2)’]
+  qspecl_then [‘λa b. ∃t. a = (bind t k1) ∧ b = (bind t k2)’]
               strip_assume_tac itree_wbisim_coind_upto >>
   pop_assum irule >>
   rw[] >-
@@ -244,7 +242,7 @@ Proof
 QED
 
 Theorem itree_bind_resp_wbisim:
-  ∀a b k1 k2. (≈ a b) ∧ (∀r. ≈ (k1 r) (k2 r)) ⇒ (≈ (⋆ a k1) (⋆ b k2))
+  ∀a b k1 k2. a ≈ b ∧ (∀r. k1 r ≈ k2 r) ⇒ bind a k1 ≈ bind b k2
 Proof
   metis_tac[itree_bind_resp_t_wbisim, itree_bind_resp_k_wbisim, itree_wbisim_trans]
 QED
@@ -254,24 +252,24 @@ QED
  *)
 
 Theorem itree_iter_ret_tau_wbisim:
-    itcb1 = (λx. case x of INL a => Tau (k1 ↻ a) | INR b => Ret b)
-  ⇒ itcb2 = (λx. case x of INL a => Tau (k2 ↻ a) | INR b => Ret b)
-  ⇒ ≈ (Ret x) (Tau u) ⇒ (∀r. ≈ (k1 r) (k2 r))
+    itcb1 = (λx. case x of INL a => Tau (iter k1 a) | INR b => Ret b)
+  ⇒ itcb2 = (λx. case x of INL a => Tau (iter k2 a) | INR b => Ret b)
+  ⇒ Ret x ≈ Tau u ⇒ (∀r. k1 r ≈ k2 r)
   ⇒ (∃t2 t3.
-      ⋆ (Ret x) itcb1 = Tau t2 ∧ ⋆ (Tau u) itcb2 = Tau t3 ∧
-      ((∃sa sb. ≈ sa sb ∧ t2 = ⋆ sa itcb1 ∧ t3 = ⋆ sb itcb2) ∨ ≈ t2 t3)) ∨
+      bind (Ret x) itcb1 = Tau t2 ∧ bind (Tau u) itcb2 = Tau t3 ∧
+      ((∃sa sb. sa ≈ sb ∧ t2 = bind sa itcb1 ∧ t3 = bind sb itcb2) ∨ t2 ≈ t3)) ∨
     (∃e k k'.
-      strip_tau (⋆ (Ret x) itcb1) (Vis e k) ∧
-      strip_tau (⋆ (Tau u) itcb2) (Vis e k') ∧
-      ∀r. (∃sa sb. ≈ sa sb ∧ k r = ⋆ sa itcb1 ∧ k' r = ⋆ sb itcb2) ∨
-          ≈ (k r) (k' r)) ∨
-    ∃r. strip_tau (⋆ (Ret x) itcb1) (Ret r) ∧
-        strip_tau (⋆ (Tau u) itcb2) (Ret r)
+      strip_tau (bind (Ret x) itcb1) (Vis e k) ∧
+      strip_tau (bind (Tau u) itcb2) (Vis e k') ∧
+      ∀r. (∃sa sb. sa ≈ sb ∧ k r = bind sa itcb1 ∧ k' r = bind sb itcb2) ∨
+          k r ≈ k' r) ∨
+    ∃r. strip_tau (bind (Ret x) itcb1) (Ret r) ∧
+        strip_tau (bind (Tau u) itcb2) (Ret r)
 Proof
   rpt strip_tac >>
   rw[itree_bind_thm] >>
-  qabbrev_tac ‘itcb1 = (λx. case x of INL a => Tau (k1 ↻ a) | INR b => Ret b)’ >>
-  qabbrev_tac ‘itcb2 = (λx. case x of INL a => Tau (k2 ↻ a) | INR b => Ret b)’ >>
+  qabbrev_tac ‘itcb1 = (λx. case x of INL a => Tau (iter k1 a) | INR b => Ret b)’ >>
+  qabbrev_tac ‘itcb2 = (λx. case x of INL a => Tau (iter k2 a) | INR b => Ret b)’ >>
   fs[Once itree_wbisim_cases] >> fs[Once $ GSYM itree_wbisim_cases] >>
   qpat_x_assum ‘strip_tau _ _’ mp_tac >>
   Induct_on ‘strip_tau’ >>
@@ -296,12 +294,12 @@ Proof
 QED
 
 Theorem itree_iter_resp_wbisim:
-  ∀t k1 k2. (∀r. ≈ (k1 r) (k2 r)) ⇒ (≈ (k1 ↻ t) (k2 ↻ t))
+  ∀t k1 k2. (∀r. k1 r ≈ k2 r) ⇒ iter k1 t ≈ iter k2 t
 Proof
   rpt strip_tac >>
-  qabbrev_tac ‘itcb1 = (λx. case x of INL a => Tau (k1 ↻ a) | INR b => Ret b)’ >>
-  qabbrev_tac ‘itcb2 = (λx. case x of INL a => Tau (k2 ↻ a) | INR b => Ret b)’ >>
-  qspecl_then [‘λia ib. ∃sa sb x. (≈ sa sb) ∧ ia = ⋆ sa itcb1 ∧ ib = ⋆ sb itcb2’]
+  qabbrev_tac ‘itcb1 = (λx. case x of INL a => Tau (iter k1 a) | INR b => Ret b)’ >>
+  qabbrev_tac ‘itcb2 = (λx. case x of INL a => Tau (iter k2 a) | INR b => Ret b)’ >>
+  qspecl_then [‘λia ib.∃sa sb x. sa ≈ sb ∧ ia = bind sa itcb1 ∧ ib = bind sb itcb2’]
               strip_assume_tac itree_wbisim_strong_coind >>
   pop_assum irule >>
   rw[] >-
@@ -311,7 +309,7 @@ Proof
       gvs[] >>
       Cases_on ‘x’ >-
        (or1_tac >> (* Ret INL by wbisim *)
-        qexistsl_tac [‘⋆ (k1 x') itcb1’, ‘⋆ (k2 x') itcb2’] >>
+        qexistsl_tac [‘bind (k1 x') itcb1’, ‘bind (k2 x') itcb2’] >>
         qunabbrev_tac ‘itcb1’ >> qunabbrev_tac ‘itcb2’ >>
         simp[Once itree_iter_thm, itree_bind_thm] >>
         simp[Once itree_iter_thm, itree_bind_thm] >>
@@ -321,7 +319,7 @@ Proof
         rw[Once itree_iter_thm, itree_bind_thm])) >-
      (irule itree_iter_ret_tau_wbisim >> metis_tac[]) >-
      (fs[Once itree_wbisim_cases]) >-
-     (‘≈ (Ret x) (Tau u)’ by fs[itree_wbisim_sym] >>
+     (‘Ret x ≈ Tau u’ by fs[itree_wbisim_sym] >>
       (* (pure)_rewrite_tac more basic *)
       rpt $ qpat_x_assum ‘Abbrev _’
           $ assume_tac o PURE_REWRITE_RULE[markerTheory.Abbrev_def] >>
@@ -337,12 +335,12 @@ Proof
       metis_tac[itree_wbisim_tau_eq, itree_wbisim_sym, itree_wbisim_trans]) >-
      (rw[itree_bind_thm] >>
       fs[Once itree_wbisim_cases] >> fs[Once $ GSYM itree_wbisim_cases] >>
-      qexists_tac ‘(λx. ⋆ (k x) itcb1)’ >>
+      qexists_tac ‘(λx. bind (k x) itcb1)’ >>
       metis_tac[itree_bind_vis_strip_tau]) >-
      (fs[Once itree_wbisim_cases]) >-
      (rw[itree_bind_thm] >>
       fs[Once itree_wbisim_cases] >> fs[Once $ GSYM itree_wbisim_cases] >>
-      qexists_tac ‘(λx. ⋆ (k' x) itcb2)’ >>
+      qexists_tac ‘(λx. bind (k' x) itcb2)’ >>
       metis_tac[itree_bind_vis_strip_tau]) >-
      (or2_tac >>
       simp[Once itree_bind_thm] >>
@@ -403,6 +401,9 @@ QED
 
 (* looping vis nodes *)
 
+open arithmeticTheory;
+open stringLib;
+
 Definition iterate_def:
   iterate emit succ zero =
   itree_unfold (λs'. Vis' (emit s') (λ_. (succ s'))) zero
@@ -462,16 +463,38 @@ Proof
 QED
 
 Theorem even_spec_thm:
-  even_spec 0 = ⋆ (⋆ (trigger "even")
-                     (λ_. (trigger "odd")))
+  even_spec 0 = bind (bind (emit "even")
+                     (λ_. (emit "odd")))
                   (λ_. even_spec 0)
 Proof
   rw[Once even_spec_unfold] >>
-  rw[itree_bind_trigger] >>
+  rw[itree_bind_emit] >>
   rw[itree_bind_thm] >>
   rw[FUN_EQ_THM] >>
-  rw[itree_bind_trigger] >>
+  rw[itree_bind_emit] >>
   rw[FUN_EQ_THM] >>
   qspec_then ‘0’ mp_tac even_spec_plus2 >>
   rw[]
 QED
+
+(* open ASCIInumbersTheory; *)
+
+Definition even_prog_def:
+  even_prog =
+  Vis "hi, input nuber:"
+      (λk. iter (λs. Vis (if EVEN s then "even" else "odd") (λ_. Ret (INL (s+1))))
+                k)
+End
+
+(* even is a constraint on event responses *)
+(* should use do notation later for clarity *)
+(* Theorem even_prog_spec: *)
+(*   ∃prelude loop coda. even_prog = bind (bind prelude loop) coda *)
+(*   ∧ prelude = emit "hi, input nuber:" *)
+(*   ∧ EVEN k ⇒ loop k ≈ (if (k = 100) *)
+(*                        then (Ret r) *)
+(*                        else (Vis "even" (λ_. Vis "odd" (λ_. loop k)))) *)
+(*   ∧ coda r = emit (CONCAT [(n2s r) , "bye"]) *)
+(* Proof *)
+(*   cheat *)
+(* QED *)
